Reduce cheats

compiler/backend/proofs/word_depthProofScript.sml
@@ -135,28 +135,51 @@ Definition max_depth_graphs_def:
     case lookup n all_funs of
     | NONE => NONE
     | SOME (a,body) =>
-        OPTION_MAP2 MAX (max_depth ss (call_graph funs n all (size all_funs) body))
-                        (max_depth_graphs ss ns all funs all_funs)
+        OPTION_MAP2 MAX (lookup n ss)
+       (OPTION_MAP2 MAX (max_depth ss (call_graph funs n all (size all_funs) body))
+                        (max_depth_graphs ss ns all funs all_funs))
 End
 
-(*
-Theorem max_depth_graphs_adjust:
-  !ns all funs c1 c2 ss.
-    subspt c1 c2 /\ set ns ⊆ domain c1 ==>
-    max_depth_graphs ss ns all funs c2 =
-    max_depth_graphs ss ns all funs c1
-Proof
-  Induct \\ fs [max_depth_graphs_def]
-  \\ rw [] \\ fs [domain_lookup]
-  \\ PairCases_on `v` \\ fs []
-  \\ fs [subspt_lookup] \\ res_tac \\ fs []
-QED
-*)
-
 Theorem MEM_max_depth_graphs:
-  MEM name ns ==>
-  option_le (max_depth_graphs ss [name] xs funs code)
-            (max_depth_graphs ss ns xs funs code)
+  !ns name y.
+    MEM name ns /\ lookup name code = SOME y ==>
+    option_le (max_depth_graphs ss [name] xs funs code)
+              (max_depth_graphs ss ns xs funs code)
+Proof
+  Induct \\ fs [] \\ rw []
+  \\ fs [max_depth_graphs_def]
+  THEN1
+   (TOP_CASE_TAC \\ fs []
+    \\ Cases_on `lookup h ss` THEN1 fs [OPTION_MAP2_DEF]
+    \\ Cases_on `max_depth ss (call_graph funs h xs (size code) r)`
+    THEN1 fs [OPTION_MAP2_DEF]
+    \\ Cases_on `max_depth_graphs ss ns xs funs code`
+    \\ fs [OPTION_MAP2_DEF])
+  \\ first_x_assum drule \\ fs []
+  \\ PairCases_on `y` \\ fs []
+  \\ Cases_on `lookup h code` THEN1 fs [OPTION_MAP2_DEF] \\ fs []
+  \\ PairCases_on `x` \\ fs []
+  \\ Cases_on `lookup h ss` THEN1 fs [OPTION_MAP2_DEF] \\ fs []
+  \\ Cases_on `max_depth_graphs ss ns xs funs code`
+  THEN1 fs [OPTION_MAP2_DEF] \\ fs []
+  \\ Cases_on `max_depth ss (call_graph funs name xs (size code) y1)`
+  THEN1 fs [OPTION_MAP2_DEF] \\ fs []
+  \\ Cases_on `max_depth ss (call_graph funs h xs (size code) x1)`
+  THEN1 fs [OPTION_MAP2_DEF] \\ fs []
+  \\ Cases_on `lookup name ss` THEN1 fs [OPTION_MAP2_DEF] \\ fs []
+QED
+
+Theorem option_le_max_depth_graphs:
+  set ns2 SUBSET set ns1 ==>
+  option_le (max_depth_graphs ss ns ns1 funs funs2)
+            (max_depth_graphs ss ns ns2 funs funs2)
+Proof
+  cheat
+QED
+
+Theorem LENGTH_LESS_size:
+  ~MEM name ns /\ set ns ⊆ domain funs ==>
+  LENGTH ns < size funs
 Proof
   cheat
 QED
@@ -166,7 +189,7 @@ Theorem max_depth_call_graph_lemma:
     evaluate (prog, s) = (res,s1) /\
     subspt funs funs2 /\ subspt funs2 s.code /\
     s.locals_size = lookup n s.stack_size /\ res <> SOME Error /\
-    MEM n ns /\ set ns SUBSET domain s.code ==>
+    MEM n ns /\ set ns SUBSET domain funs2 ==>
     option_le s1.stack_max
       (OPTION_MAP2 MAX s.stack_max
         (OPTION_MAP2 (+) (stack_size s.stack)
@@ -179,7 +202,6 @@ Theorem max_depth_call_graph_lemma:
      (res = NONE ==> s1.locals_size = s.locals_size))
 
 Proof
-
   recInduct evaluate_ind \\ rpt conj_tac \\ rpt gen_tac \\ strip_tac
   THEN1 (* Skip *)
    (fs [wordSemTheory.evaluate_def] \\ rveq
@@ -277,7 +299,7 @@ Proof
     \\ imp_res_tac evaluate_code_only_grows
     \\ `subspt funs s0.code` by imp_res_tac subspt_trans
     \\ first_x_assum (qspecl_then [`funs`,`n`,`ns`,`funs2`] mp_tac)
-    \\ `set ns SUBSET domain s0.code /\ subspt funs2 s0.code` by
+    \\ `set ns SUBSET domain funs2 /\ subspt funs2 s0.code` by
      (imp_res_tac evaluate_code_only_grows
       \\ fs [SUBSET_DEF,domain_lookup,subspt_lookup]
       \\ rw [] \\ res_tac \\ fs [] \\ res_tac \\ fs [])
@@ -360,11 +382,8 @@ Proof
   \\ TOP_CASE_TAC \\ simp []
   \\ rename [`lookup name funs = SOME (a,body)`]
   \\ TOP_CASE_TAC \\ simp []
-
   THEN1 (* ret = NONE i.e. tail-call *)
-   (
-
-    Cases_on `MEM name ns` \\ fs []
+   (Cases_on `MEM name ns` \\ fs []
     THEN1
      (simp [evaluate_def,CaseEq"option",CaseEq"bool",pair_case_eq,find_code_def]
       \\ Cases_on `res = SOME Error` \\ asm_rewrite_tac []
@@ -385,8 +404,7 @@ Proof
        (match_mp_tac backendPropsTheory.option_le_trans
         \\ qexists_tac `max_depth_graphs s.stack_size [name] ns funs funs2`
         \\ reverse conj_tac THEN1 (match_mp_tac MEM_max_depth_graphs \\ fs [])
-        \\ fs [max_depth_graphs_def,OPTION_MAP2_MAX_SOME_0]
-        \\ cheat (* tweak def *))
+        \\ fs [max_depth_graphs_def,OPTION_MAP2_MAX_SOME_0])
       \\ qmatch_assum_abbrev_tac `option_le (_ _ x1) x2`
       \\ Cases_on `x2` THEN1 fs [OPTION_MAP2_DEF]
       \\ Cases_on `x1` THEN1 fs [OPTION_MAP2_DEF]
@@ -396,7 +414,9 @@ Proof
       \\ Cases_on `stack_size s.stack` THEN1 fs [OPTION_MAP2_DEF]
       \\ Cases_on `s'.stack_max` THEN1 fs [OPTION_MAP2_DEF]
       \\ fs [])
-    \\ `LENGTH ns < size funs2` by cheat \\ asm_rewrite_tac []
+    \\ Cases_on `set ns ⊆ domain funs2` \\ fs []
+    \\ `LENGTH ns < size funs2` by (imp_res_tac LENGTH_LESS_size \\ fs [])
+    \\ asm_rewrite_tac []
     \\ fs [evaluate_def,CaseEq"option",CaseEq"bool",pair_case_eq,find_code_def]
     \\ Cases_on `res = SOME Error` \\ fs [PULL_EXISTS]
     \\ rpt gen_tac \\ strip_tac \\ rveq \\ fs []
@@ -405,7 +425,7 @@ Proof
     \\ first_x_assum (qspecl_then [`funs`,`name`,`name::ns`,`funs2`] mp_tac)
     \\ impl_tac
     THEN1 (fs [subspt_lookup,lookup_delete] \\ rw []
-           \\ fs [call_env_def,domain_lookup])
+           \\ fs [call_env_def,domain_lookup] \\ res_tac \\ fs [])
     \\ fs [subspt_lookup,lookup_delete] \\ res_tac \\ fs []
     \\ rveq \\ fs []
     \\ fs [max_depth_mk_Branch,max_depth_def,OPTION_MAP2_ADD_SOME_0]
@@ -420,7 +440,8 @@ Proof
     \\ fs [subspt_lookup] \\ res_tac \\ fs [] \\ rveq
     \\ `option_le
          (max_depth_graphs s.stack_size ns (name::ns) funs funs2)
-         (max_depth_graphs s.stack_size ns ns funs funs2)` by cheat
+         (max_depth_graphs s.stack_size ns ns funs funs2)` by
+      (match_mp_tac option_le_max_depth_graphs \\ fs [] \\ rw [])
     \\ qmatch_assum_abbrev_tac `option_le x1 x2`
     \\ Cases_on `x2` THEN1 fs [OPTION_MAP2_DEF]
     \\ Cases_on `x1` THEN1 fs [OPTION_MAP2_DEF]
@@ -466,7 +487,7 @@ Proof
       \\ first_x_assum (qspecl_then [`delete name funs`,
            `name`,`[name]`,`funs2`] mp_tac)
       \\ impl_tac THEN1 (fs [subspt_lookup,lookup_delete]
-                         \\ fs [call_env_def,domain_lookup])
+                         \\ fs [call_env_def,domain_lookup] \\ res_tac \\ fs [])
       \\ fs [max_depth_graphs_def,OPTION_MAP2_MAX_SOME_0,OPTION_MAP2_simps]
       \\ fs [push_env_def] \\ pairarg_tac \\ fs []
       \\ fs [dec_clock_def,call_env_def]
@@ -495,6 +516,14 @@ Proof
   \\ cheat
 QED
 
+Definition full_call_graph_def:
+  full_call_graph n funs =
+    case lookup n funs of
+    | NONE => Unknown
+    | SOME (a,prog) => Branch (Call n Leaf)
+                         (call_graph funs n [n] (size funs) prog)
+End
+
 Theorem max_depth_call_graph:
   !prog s res s1 funs n a.
     lookup n funs = SOME (a,prog) /\
@@ -503,13 +532,15 @@ Theorem max_depth_call_graph:
     option_le s1.stack_max
       (OPTION_MAP2 MAX s.stack_max
         (OPTION_MAP2 (+) (stack_size s.stack)
-          (max_depth s.stack_size (call_graph funs n [n] (size funs) prog))))
+          (max_depth s.stack_size (full_call_graph n funs))))
 Proof
-  rw [] \\ drule max_depth_call_graph_lemma
+  rw [full_call_graph_def] \\ drule max_depth_call_graph_lemma
   \\ disch_then (qspecl_then [`funs`,`n`,`[n]`,`funs`] mp_tac)
   \\ fs [domain_lookup]
   \\ fs [max_depth_graphs_def,OPTION_MAP2_simps,OPTION_MAP2_MAX_SOME_0]
   \\ fs [subspt_lookup] \\ res_tac \\ fs []
+  \\ fs [GSYM OPTION_MAP2_MAX_ASSOC,OPTION_MAP2_simps,max_depth_def,
+         OPTION_MAP2_ADD_SOME_0]
 QED
 
 val _ = export_theory();
